Use inode type to record allocation
Don't actually need inode bitmaps; using the type is vastly simpler, and
we're already recording file vs directory directly in the inode.

In the process I also cleaned up the invariant so that it's heavily
based on inode type (lining up nicely which the code, which typically
first discriminates based on type). Some more careful modifies and reads
clauses also let us reveal a lot fewer definitions by showing that the
low-level modifications to the lowest-level fs (fs.fs.fs unfortunately
in dir_fs.dfy), which are common due to startInode/finishInode, have no
impact on most of the validity predicate.

src/Dafny/examples/fs/dir_fs.dfy
@@ -9,6 +9,7 @@ module DirFs
   import opened FsKinds
   import opened JrnlTypes
   import opened JrnlSpec
+  import opened Alloc
 
   import opened DirEntries
   import opened ByteFs
@@ -48,38 +49,79 @@ module DirFs
     // domain is just the inodes that are allocated directories
     ghost var dirents: map<Ino, Dirents>
     const fs: ByteFilesys<()>
-    const rootIno: Ino
+    const ialloc: MaxAllocator
 
-    const Repr: set<object> := {this} + fs.Repr
+    static const rootIno: Ino := 1 as Ino;
 
-    static predicate alloc_ino_dom<T>(inode_owner: map<Ino, Option<()>>, m: map<Ino, T>)
-      requires ino_dom(inode_owner)
+    const Repr: set<object> := {this} + fs.Repr + ialloc.Repr
+
+    static const iallocMax: uint64 := super.num_inodes as uint64 - 8
+
+    predicate is_invalid(ino: Ino) reads this
+    { ino !in data && ino !in dirents }
+
+    predicate is_file(ino: Ino) reads this
+    { ino in data && ino !in dirents && data[ino].ByteFile? }
+
+    predicate is_dir(ino: Ino) reads this
+    { ino in data && ino in dirents && data[ino].DirFile? }
+
+    predicate {:opaque} is_of_type(ino: Ino, t: Inode.InodeType)
+      reads this
     {
-      forall ino:Ino :: ino in m <==> inode_owner[ino].Some?
+      && (t.InvalidType? ==> is_invalid(ino))
+      && (t.FileType? ==> is_file(ino))
+      && (t.DirType? ==> is_dir(ino))
     }
 
-    predicate ValidDomains()
+    predicate ValidTypes()
+      reads this, fs.fs
+      requires Fs.ino_dom(fs.fs.metadata)
+    {
+      forall ino: Ino :: is_of_type(ino, fs.inode_types()[ino])
+    }
+
+    lemma type_invert(ino: Ino)
       requires fs.fs.Valid()
-      reads Repr
+      requires ValidTypes()
+      ensures ino !in data ==> fs.inode_types()[ino].InvalidType? && ino !in dirents
+      ensures ino in data && data[ino].ByteFile? ==> fs.inode_types()[ino].FileType? && ino !in dirents
+      ensures ino in dirents ==> fs.inode_types()[ino].DirType? && ino in data
     {
-      && alloc_ino_dom(fs.fs.inode_owner(), data)
-      && (forall ino:Ino :: ino in dirents <==>
-        fs.inode_types()[ino].DirType?)
+      var t := fs.inode_types()[ino];
+      assert is_of_type(ino, t);
+      reveal is_of_type();
+      if t.InvalidType? { return; }
+      if t.FileType? { return; }
+      if t.DirType? { return; }
+      assert false;
     }
+
+    predicate ValidAlloc()
+      reads ialloc.Repr, fs.Repr
+    {
+      && ialloc.Valid()
+      && ialloc.max == iallocMax
+      && ialloc.Repr !! fs.Repr
+    }
+
+    twostate lemma ValidAlloc_monotonic()
+      requires old(ValidAlloc())
+      ensures ValidAlloc()
+    {}
 
     predicate {:opaque} ValidRoot()
-      reads Repr
-      requires fs.fs.Valid()
+      reads this, fs.fs
+      requires Fs.ino_dom(fs.fs.metadata)
     {
-      // the root inode is allocated and is actually a directory
-      && fs.fs.inode_owner()[rootIno].Some?
+      // the root inode is actually a directory
       && fs.inode_types()[rootIno].DirType?
       && rootIno != 0
     }
 
     predicate ValidDirents()
       requires fs.fs.Valid()
-      reads Repr
+      reads this, fs.Repr
     {
       forall ino:Ino | ino in dirents ::
         fs.data()[ino] == dirents[ino].enc()
@@ -87,26 +129,23 @@ module DirFs
 
     predicate {:opaque} ValidFiles()
       requires fs.fs.Valid()
-      reads Repr
+      reads this, fs.Repr
     {
-      forall ino:Ino | fs.fs.inode_owner()[ino].Some? && fs.inode_types()[ino].FileType? ::
-           ino in data && data[ino] == ByteFile(fs.data()[ino])
+      forall ino:Ino | is_file(ino) ::
+        data[ino] == ByteFile(fs.data()[ino])
     }
 
     predicate {:opaque} ValidDirs()
-      requires fs.fs.Valid()
-      reads Repr
+      reads this
     {
 
-      && (forall ino:Ino | ino in dirents :: ino in data &&
-        data[ino] == DirFile(dirents[ino].dir))
-      && (forall ino:Ino :: fs.inode_types()[ino].DirType? ==>
-        fs.fs.inode_owner()[ino].Some?)
+      forall ino:Ino | is_dir(ino) ::
+        data[ino] == DirFile(dirents[ino].dir)
     }
 
     predicate ValidData()
       requires fs.fs.Valid()
-      reads Repr
+      reads this, fs.Repr
     {
       && ValidFiles()
       && ValidDirs()
@@ -114,17 +153,17 @@ module DirFs
 
     predicate ValidUnusedInodes()
       requires fs.fs.Valid()
-      reads Repr
+      reads this, fs.Repr
     {
-      forall ino:Ino | fs.fs.inode_owner()[ino].None? ::
-        fs.inode_types()[ino].FileType? && fs.data()[ino] == []
+      forall ino:Ino | is_invalid(ino) :: fs.data()[ino] == []
     }
 
     predicate ValidDirFs()
       requires fs.fs.Valid()
       reads Repr
     {
-      && ValidDomains()
+      && ValidTypes()
+      && ValidAlloc()
       && ValidRoot()
       && ValidDirents()
       && ValidData()
@@ -145,21 +184,21 @@ module DirFs
       && ValidDirFs()
     }
 
-    constructor Init(fs: ByteFilesys<()>, rootIno: Ino)
+    constructor Init(fs: ByteFilesys<()>)
       requires fs.Valid()
       requires fs.data() == map ino: Ino {:trigger} :: if ino == rootIno then Dirents.zero.enc() else []
-      requires fs.inode_types() == map ino: Ino {:trigger} :: if ino == rootIno then Inode.DirType else Inode.FileType
-      requires fs.fs.inode_owner() == map ino: Ino {:trigger} :: if ino == rootIno then Fs.Some(()) else Fs.None
-      requires rootIno != 0
+      requires fs.inode_types() == map ino: Ino {:trigger} :: if ino == rootIno then Inode.DirType else Inode.InvalidType
       ensures Valid()
       ensures this.rootIno == rootIno
       ensures data == map[rootIno := File.emptyDir]
     {
       this.fs := fs;
-      this.rootIno := rootIno;
       var dirents0 : map<Ino, Dirents> := map[rootIno := Dirents.zero];
       this.dirents := dirents0;
       this.data := map[rootIno := File.emptyDir];
+      var ialloc := new MaxAllocator(iallocMax);
+      ialloc.MarkUsed(rootIno);
+      this.ialloc := ialloc;
       new;
       Dirents.zero_dir();
       assert ValidData() by {
@@ -167,27 +206,19 @@ module DirFs
         reveal ValidDirs();
       }
       assert ValidRoot() by { reveal ValidRoot(); }
+      assert ValidTypes() by { reveal is_of_type(); }
     }
 
-    static method allocEmptyDir(fs: ByteFilesys<()>, txn: Txn) returns (ok: bool, ino: Ino)
+    static method createRootDir(fs: ByteFilesys<()>, txn: Txn) returns (ok: bool)
       modifies fs.Repr
       requires fs.Valid() ensures ok ==> fs.Valid()
       requires fs.fs.has_jrnl(txn)
       requires forall ino:Ino :: fs.data()[ino] == []
       ensures ok ==>
-      && ino != 0
-      && fs.data() == old(fs.data()[ino := Dirents.zero.enc()])
-      && old(fs.fs.inode_owner()[ino].None?)
-      && fs.fs.inode_owner() == old(fs.fs.inode_owner()[ino := Some(())])
-      && fs.inode_types() == old(fs.inode_types()[ino := Inode.DirType])
+      && fs.data() == old(fs.data()[rootIno := Dirents.zero.enc()])
+      && fs.inode_types() == old(fs.inode_types()[rootIno := Inode.DirType])
     {
-      ok, ino := fs.allocInode(txn, ());
-      var ino0 := ino;
-      if !ok {
-        return;
-      }
-
-      assert fs.Valid();
+      var ino := rootIno;
 
       var i := fs.startInode(txn, ino);
       i := fs.setType(ino, i, Inode.DirType);
@@ -210,7 +241,7 @@ module DirFs
       var fs_ := new ByteFilesys.Init(d);
 
       var txn := fs_.jrnl.Begin();
-      var ok, rootIno_ := allocEmptyDir(fs_, txn);
+      var ok := createRootDir(fs_, txn);
       if !ok {
         return None;
       }
@@ -220,62 +251,75 @@ module DirFs
       }
       assert fs_.Valid();
 
-      var dir_fs := new DirFilesys.Init(fs_, rootIno_);
+      var dir_fs := new DirFilesys.Init(fs_);
       return Some(dir_fs);
     }
 
-    lemma alloc_ino_dom_not<T>(inode_owner: map<Ino, Option<()>>, m: map<Ino, T>, ino: Ino)
-      requires ino_dom(inode_owner)
-      requires alloc_ino_dom(inode_owner, m)
-      requires !inode_owner[ino].Some?
-      ensures ino !in m
-    {}
-
-    method {:timeLimitMultiplier 2} readDirents(txn: Txn, d_ino: Ino)
-      returns (err: Error, dents: Dirents)
+    method startInode(txn: Txn, ino: Ino)
+      returns (i: Inode.Inode)
       modifies fs.fs.fs
-      requires Valid() ensures Valid()
       requires fs.fs.has_jrnl(txn)
-      ensures err.NoError? ==> d_ino in dirents && dents == dirents[d_ino]
-      ensures err.DoesNotExist? ==> d_ino !in data
-      ensures err.NotADir? ==> d_ino in data && data[d_ino].ByteFile?
-      ensures !err.IsADir?
+      requires Valid()
+      ensures ValidIno(ino, i) && i.meta.ty == fs.inode_types()[ino]
+      ensures fs.fs.fs.cur_inode == Fs.Some( (ino, i) )
+      ensures data == old(data)
+      ensures dirents == old(dirents)
+      ensures fs.types_unchanged()
     {
-      var i := fs.startInode(txn, d_ino);
-      fs.inode_metadata(d_ino, i);
-      var dir_exists? := fs.fs.fs.isInodeAllocated(txn, d_ino);
-      if !dir_exists? {
-        fs.finishInodeReadonly(d_ino, i);
-        assert ValidData() by {
-          reveal ValidFiles();
-          reveal ValidDirs();
-        }
-        assert ValidRoot() by { reveal ValidRoot(); }
-        err := DoesNotExist;
-        return;
-      }
-      if i.meta.ty == Inode.FileType {
-        fs.finishInodeReadonly(d_ino, i);
-        err := NotADir;
+      i := fs.startInode(txn, ino);
+      fs.inode_metadata(ino, i);
+      assert ValidData() by {
         reveal ValidFiles();
-        reveal ValidDirs();
-        assert ValidRoot() by { reveal ValidRoot(); }
-        return;
       }
-      err := NoError;
-      assert d_ino in dirents;
+    }
 
+    method readDirentsInode(txn: Txn, d_ino: Ino, i: Inode.Inode)
+      returns (dents: Dirents)
+      requires ValidIno(d_ino, i)
+      requires fs.fs.has_jrnl(txn)
+      requires is_dir(d_ino)
+      ensures dents == dirents[d_ino]
+    {
       assert |fs.data()[d_ino]| == 4096 by {
         dirents[d_ino].enc_len();
       }
       var bs := fs.readInternal(txn, d_ino, i, 0, 4096);
-      fs.finishInodeReadonly(d_ino, i);
       dents := Dirents.decode(bs, dirents[d_ino]);
+    }
+
+    method readDirents(txn: Txn, d_ino: Ino)
+      returns (err: Error, dents: Dirents)
+      modifies fs.fs.fs
+      requires Valid() ensures Valid()
+      requires fs.fs.has_jrnl(txn)
+      ensures err.NoError? ==> is_dir(d_ino) && dents == dirents[d_ino]
+      ensures err.DoesNotExist? ==> is_invalid(d_ino)
+      ensures err.NotADir? ==> is_file(d_ino)
+      ensures !err.IsADir?
+    {
+      var i := startInode(txn, d_ino);
+      if !i.meta.ty.DirType? {
+        fs.finishInodeReadonly(d_ino, i);
+        assert ValidData() by {
+          reveal ValidFiles();
+        }
+        if i.meta.ty.InvalidType? {
+          assert is_invalid(d_ino) by { reveal is_of_type(); }
+          err := DoesNotExist;
+          return;
+        }
+        // is a file
+        assert is_file(d_ino) by { reveal is_of_type(); }
+        err := NotADir;
+        return;
+      }
+      assert is_dir(d_ino) by { reveal is_of_type(); }
+      err := NoError;
+      dents := readDirentsInode(txn, d_ino, i);
+      fs.finishInodeReadonly(d_ino, i);
       assert ValidData() by {
         reveal ValidFiles();
-        reveal ValidDirs();
       }
-      assert ValidRoot() by { reveal ValidRoot(); }
     }
 
     static method writeDirentsToFs(fs: ByteFilesys<()>, txn: Txn, d_ino: Ino, dents: Dirents)
@@ -284,7 +328,6 @@ module DirFs
       requires fs.Valid() ensures fs.Valid()
       requires fs.fs.has_jrnl(txn)
       requires |fs.data()[d_ino]| == 4096
-      ensures fs.fs.inode_owner() == old(fs.fs.inode_owner())
       ensures fs.types_unchanged()
       ensures ok ==> fs.data() == old(fs.data()[d_ino := dents.enc()])
       ensures !ok ==> fs.data() == old(fs.data())
@@ -302,18 +345,17 @@ module DirFs
       assert fs.data()[d_ino] == dents.enc();
     }
 
-    method {:timeLimitMultiplier 2} writeDirents(txn: Txn, d_ino: Ino, dents: Dirents)
+    method writeDirents(txn: Txn, d_ino: Ino, dents: Dirents)
       returns (ok:bool)
       modifies Repr
       requires fs.fs.has_jrnl(txn)
       requires Valid() ensures Valid()
-      requires IsDir: d_ino in dirents
+      requires is_dir(d_ino)
       ensures ok ==>
            && dirents == old(dirents[d_ino := dents])
            && data == old(data[d_ino := DirFile(dents.dir)])
     {
       assert |fs.data()[d_ino]| == 4096 by {
-        reveal IsDir;
         dirents[d_ino].enc_len();
       }
       ok := writeDirentsToFs(fs, txn, d_ino, dents);
@@ -323,14 +365,14 @@ module DirFs
           reveal ValidDirs();
         }
         assert ValidRoot() by { reveal ValidRoot(); }
+        assert ValidTypes() by { reveal is_of_type(); }
         return;
       }
 
       dirents := dirents[d_ino := dents];
       data := data[d_ino := DirFile(dents.dir)];
 
-      reveal IsDir;
-      assert fs.inode_types()[d_ino].DirType?;
+      assert is_dir(d_ino);
       assert ValidFiles() by {
         reveal ValidFiles();
       }
@@ -338,6 +380,40 @@ module DirFs
         reveal ValidDirs();
       }
       assert ValidRoot() by { reveal ValidRoot(); }
+      assert ValidTypes() by { reveal is_of_type(); }
+    }
+
+    // allocInode finds an invalid inode and prepares it for writes
+    method allocInode(txn: Txn) returns (ok: bool, ino: Ino, i: Inode.Inode)
+      modifies fs.fs.fs, ialloc.Repr
+      requires Valid()
+      ensures ok ==> ValidIno(ino, i)
+      ensures !ok ==> Valid()
+      requires fs.fs.has_jrnl(txn)
+      ensures dirents == old(dirents)
+      ensures data == old(data)
+      ensures fs.types_unchanged()
+      ensures ok ==> old(is_invalid(ino)) && is_invalid(ino) && ino != rootIno
+      ensures ok ==> ino != 0
+    {
+      ino := ialloc.Alloc();
+      i := fs.startInode(txn, ino);
+      fs.inode_metadata(ino, i);
+      assert is_of_type(ino, i.meta.ty);
+      assert ValidIno(ino, i) by {
+        assert ValidFiles() by { reveal ValidFiles(); }
+      }
+      ok := i.meta.ty.InvalidType?;
+      if !ok {
+        fs.finishInodeReadonly(ino, i);
+        assert Valid() by {
+          assert ValidFiles() by { reveal ValidFiles(); }
+        }
+      }
+      assert ok ==> is_invalid(ino) && ino != rootIno by {
+        reveal is_of_type();
+        reveal ValidRoot();
+      }
     }
 
     // private
@@ -353,27 +429,29 @@ module DirFs
       requires fs.fs.has_jrnl(txn)
       ensures dirents == old(dirents)
       ensures ok ==>
-      && ino !in old(data)
+      && old(is_invalid(ino))
       && ino != 0
       && data == old(data[ino := File.empty])
       ensures !ok ==> data == old(data)
     {
-      ok, ino := fs.allocInode(txn, ());
+      var i;
+      ok, ino, i := this.allocInode(txn);
       if !ok {
-        assert ValidData() by {
-          reveal ValidFiles();
-          reveal ValidDirs();
-        }
-        assert ValidRoot() by { reveal ValidRoot(); }
         return;
       }
+      i := fs.setType(ino, i, Inode.FileType);
+      fs.finishInode(txn, ino, i);
       data := data[ino := File.empty];
+      assert is_of_type(ino, Inode.FileType) by {
+        reveal is_of_type();
+      }
       assert ValidDirs() by {
         reveal ValidDirs();
       }
       assert ValidFiles() by {
         reveal ValidFiles();
       }
+      assert ValidTypes() by { reveal is_of_type(); }
       assert ValidRoot() by { reveal ValidRoot(); }
     }
 
@@ -383,8 +461,8 @@ module DirFs
       requires Valid() ensures ok ==> Valid()
       requires fs.fs.has_jrnl(txn)
       ensures ok ==>
-      && d_ino in old(data) && old(data[d_ino].DirFile?)
-      && ino !in old(data)
+      && old(is_dir(d_ino))
+      && old(is_invalid(ino))
       && data == old(
         var d := data[d_ino].dir;
         var d' := DirFile(d[name := ino]);
@@ -394,9 +472,6 @@ module DirFs
       if err.IsError() {
         ok := false;
         return;
-      }
-      assert d_ino_ok: d_ino in old(data) && old(data[d_ino].DirFile?) by {
-        reveal ValidDirs();
       }
       ok, ino := allocFile(txn);
       if !ok {
@@ -426,11 +501,10 @@ module DirFs
         return;
       }
       // assert data == old(data[ino := File.empty][d_ino := DirFile(d')]);
-      reveal d_ino_ok;
       reveal ino_ok;
     }
 
-    method {:timeLimitMultiplier 2} Stat(txn: Txn, ino: Ino)
+    method Stat(txn: Txn, ino: Ino)
       returns (ok: bool, r: StatRes)
       modifies fs.fs.fs
       requires Valid() ensures Valid()
@@ -442,52 +516,36 @@ module DirFs
           && data[ino].ByteFile? ==> r.size as nat == |data[ino].data|
           && data[ino].DirFile? ==> r.size as nat == |data[ino].dir|
     {
-      var i := fs.startInode(txn, ino);
-      fs.inode_metadata(ino, i);
-      var file_exists? := fs.fs.fs.isInodeAllocated(txn, ino);
-      if !file_exists? {
+      var i := startInode(txn, ino);
+      if i.meta.ty.InvalidType? {
+        assert is_invalid(ino) by { reveal is_of_type(); }
         fs.finishInodeReadonly(ino, i);
         assert ValidData() by {
           reveal ValidFiles();
-          reveal ValidDirs();
         }
-        assert ValidRoot() by { reveal ValidRoot(); }
         ok := false;
         return;
       }
       ok := true;
-      assert ino in data;
-      var is_dir := i.meta.ty == Inode.DirType;
-      assert is_dir == data[ino].DirFile? by {
-        reveal ValidDirs();
-        reveal ValidFiles();
-      }
-      if is_dir {
-        assert |fs.data()[ino]| == 4096 by {
-          dirents[ino].enc_len();
-        }
-        var bs := fs.readInternal(txn, ino, i, 0, 4096);
+      if i.meta.ty.DirType? {
+        assert is_dir(ino) by { reveal is_of_type(); }
+        var dents := readDirentsInode(txn, ino, i);
         fs.finishInodeReadonly(ino, i);
-        var dents := Dirents.decode(bs, dirents[ino]);
         assert Valid() by {
-          assert ValidData() by {
-            reveal ValidFiles();
-            reveal ValidDirs();
-          }
-          assert ValidRoot() by { reveal ValidRoot(); }
+          assert ValidFiles() by { reveal ValidFiles(); }
         }
         var num_entries := dents.numValid();
         r := StatRes(true, num_entries);
         return;
       }
       // is a file
+      assert i.meta.ty.FileType?;
+      assert is_file(ino) by { reveal is_of_type(); }
       fs.finishInodeReadonly(ino, i);
-      r := StatRes(false, i.sz);
-      assert ValidData() by {
-        reveal ValidFiles();
-        reveal ValidDirs();
+      assert Valid() by {
+        assert ValidFiles() by { reveal ValidFiles(); }
       }
-      assert ValidRoot() by { reveal ValidRoot(); }
+      r := StatRes(false, i.sz);
       return;
     }
 
